Begining proof of mtype equal for subclasses

src/Coq/Syntax.v
@@ -5,13 +5,11 @@ Notation "'[' X ']'" := (list X) (at level 40).
 (* We will use Notation to make automation easier
  * This will be the notation to be similar with haskell *)
 
-Inductive ClassName :=
-  | ClassObject : ClassName
-  | ClassId : id -> ClassName.
+Definition ClassName := id.
+Parameter Object: ClassName.
  
-Inductive Var :=
-  | This : Var
-  | VarId: id -> Var.
+Definition Var := id.
+Parameter this: Var.
 
 Inductive Argument :=
   | Arg : id -> Argument.
@@ -21,6 +19,9 @@ Inductive Assignment :=
 
 Inductive FormalArg :=
   | FArg : ClassName -> id -> FormalArg.
+
+Definition fargType (f: FormalArg):ClassName := 
+  match f with FArg t _ => t end.
 
 Inductive Constructor :=
   | KDecl : id -> [FormalArg] -> [Argument] -> [Assignment] -> Constructor.
@@ -47,31 +48,93 @@ Inductive Program :=
 Parameter CT: @partial_map ClassDecl.
 (*We will assume a global CT to make our definitions easier
  *To instance the CT use Hypothesis x: CT = ... *)
-
+(*
 Definition extends (C D : ClassName) :=
   match C with
-  | ClassObject => None
-  | ClassId cname => find cname CT
+  | Object => None
+  | cname => find cname CT
   end.
-
-  Print extends.
-
-
+*)
 Reserved Notation "C '<:' D " (at level 40).
 
-Inductive Subtype : ClassName -> ClassName -> Set :=
+Inductive Subtype : id -> ClassName -> Set :=
   | S_Refl: forall C: ClassName, C <: C
   | S_Trans: forall (C D E: ClassName), 
     C <: D -> 
     D <: E -> 
     C <: E
-  | S_Decl: forall C D, 
-    (exists decl, extends C D = Some decl) -> 
+  | S_Decl: forall C D fs K mds , 
+    binds C (CDecl C D fs K mds) CT -> 
     C <: D
 where "C '<:' D" := (Subtype C D).
 
-Definition Bind := @partial_map Exp.
+Tactic Notation "subtype_cases" tactic(first) ident(c) :=
+  first;
+  [ Case_aux c "S_Refl" | Case_aux c "S_Trans" 
+  | Case_aux c "S_Decl"].
+  
+(* Auxiliaries *)
 
+Definition ty := ClassName.
+Definition mtyping :=  [ty] -> ty.
+
+
+Inductive fields : id -> [FieldDecl] -> Prop :=
+ | fields_obj : fields Object nil
+ | fields_other : forall C D fs K mds fs', 
+     binds C (CDecl C D fs K mds) CT ->
+     fields D fs' ->
+     fields C (fs'++fs).
+
+(*Notation "ts '~>' t" := (mtyping ts t) (at level 60).*)
+Print ty.
+
+Reserved Notation "'mtype(' m ',' D ')' '=' c '~>' c0" (at level 40).
+Inductive m_type (m: id) (C: ClassName) (B: ClassName) (ts: [ClassName]):=
+  | mty_ok : forall D Fs K Ms e fargs,
+              binds C (CDecl C D Fs K Ms) CT->
+              List.In (MDecl B m fargs e) Ms ->
+              map fargType fargs = ts ->
+              mtype(m, C) = B ~> ts
+  | mty_no_override: forall D Fs K Ms e fargs,
+              binds C (CDecl C D Fs K Ms) CT->
+              ~List.In (MDecl B m fargs e) Ms ->
+              mtype(m, D) = B ~> ts ->
+              mtype(m,C) = B ~> ts
+  where "'mtype(' m ',' D ')' '=' c '~>' c0"
+        := (m_type m D c c0).
+
+Hint Constructors m_type.
+
+Lemma A11: forall m D C Cs C0,
+          C <: D ->
+          mtype(m,D) = Cs ~> C0 ->
+          mtype(m,C) = Cs ~> C0.
+Proof.
+  intros m D C Cs C0 H.
+  subtype_cases (induction H) Case; auto.
+  Case "S_Decl".
+    intros.
+    inversion H. subst.
+    eapply mty_ok; eauto.
+    intro. (*we need to assume that the CT is consistent*)
+    contradiction.
+    constructor.
+    inversion b.
+    inversion H1.
+    
+
+    
+
+
+  
+
+Lemma A11 : forall C D m, 
+    C <: D -> 
+    mtype m D = t -> 
+    mtype m C = t.
+
+Definition Bind := @partial_map Exp.
 
 Lemma eq_var_dec : forall (v v': Var), {v = v'} + {v <> v'}.
 Proof.
@@ -91,7 +154,7 @@ Proof.
       inversion H. auto.
 Defined.
 
-Fixpoint subst (e: Exp) (v: Var) (v': Exp) :=
+Fixpoint subst (e: Exp) (v: Var) (v': Exp) : Exp:=
   match e with
   | ExpVar var => if eq_var_dec var v then v' else ExpVar var
   | ExpFieldAccess exp i => ExpFieldAccess (subst exp v v') i
@@ -104,4 +167,6 @@ Fixpoint subst (e: Exp) (v: Var) (v': Exp) :=
 Notation " '[' v ':=' v' ']' e " := (subst e v v') (at level 40).  
 
 Eval compute in ([ (VarId (Id 1)) := ExpFieldAccess (ExpVar This) (Id 2)] ExpVar (VarId (Id 1))).
+
+
 
